\documentclass{article}
\usepackage{amsmath, amsthm, amssymb}
\usepackage{tikz}
\usepackage{array}
\usepackage{graphicx} % Added for including the PDF file as an image
\usepackage{float}
\usepackage{mathpazo}
\usetikzlibrary{angles, quotes}

\begin{document}
\section*{\huge Mathematics Homework Sheet 9}
\begin{flushright}
   \textbf{Authors: Abdullah Oguz Topcuoglu \& Ahmed Waleed Ahmed Badawy Shora}
\end{flushright}


% 1. Construct a 4 × 4 real matrix D such that
% ker D =
% *
% 
% 
% 0
% 1
% 0
% 0
% 
%  ,
% 
% 
% 0
% 0
% 1
% 0
% 
% 
% +
% , Im D =
% *
% 
% 
% 1
% 1
% 1
% 1
% 
%  ,
% 
% 
% 0
% 1
% 1
% 1
% 
% 
% +
% .
% [Hint: D = (De1|De2|De3|De4) and Im D = ⟨De1, De2, De3, De4⟩.]
% 2. Find all real nontrivial solutions of the equations
% 2x1 − 3x2 − x3 + x4 = 0,
% 3x1 + 4x2 − 4x3 − 3x4 = 0,
% 17x2 − 5x3 − 9x4 = 0.
% Show that one of these solutions satisfies the equations
% x1 + x2 + x3 + x4 + 1 = 0,
% x1 − x2 − x3 − x4 − 3 = 0
% but none can be written as a linear combination of the vectors (0, 1, 2, 3) and (3, 2, 1, 0).
% 3. Show that
% det
% 
% 
% a
% 2 + 1 ab ac
% ab b2 + 1 bc
% ac bc c2 + 1
% 
%  = a
% 2 + b
% 2 + c
% 2 + 1.
% 4. Let K be a field.
% (a) Two matrices A, B = Kn×n are called similar if there is a matrix P ∈ GL(n, K) such
% that B = P
% −1AP. Prove that
% (i) similarity of matrices defines an equivalence relation ∼ on Kn×n
% ,
% (ii) A ∼ B if and only if there is a finite-dimensional vector space V over K with bases
% B, B
% ′ and a linear transformation T : V → V such that A = MB
% B
% (T), B = MB
% ′
% B′(T).
% (b) Prove that two similar matrices have the same determinant.
% (c) Let V be an n-dimensional vector space over K. How would you define the determinant
% of a linear transformation T : V → V ?
% 5. Which of the matrices
% 
% −3 4
% −1 1
% ,
% 
% −3 1
% −2 −1
% 
% ,
% 
% −3 3
% 2 −2
% 
% ,
% 
% 2 −1
% −1 3 
% are diagonalisable over Q, R or C?


\section*{Problem 1}
From the given hint i observe that the columns of the matrix is just the images of the standard basis vectors.
And since \(e_2\) and \(e_3\) are in the kernel, second and third columns of \(D\) are all zeros.
\begin{align*}
D = \begin{pmatrix}
x & 0 & 0 & x \\
x & 0 & 0 & x \\
x & 0 & 0 & x \\
x & 0 & 0 & x
\end{pmatrix}
\end{align*}

And also from the hint i observe that the image is just span of the column vectors of the matrix. So i will just plug the given vectors in the image of \(D\)
into the columns of \(D\)
\begin{align*}
D = \begin{pmatrix}
1 & 0 & 0 & 0 \\
1 & 0 & 0 & 1 \\
1 & 0 & 0 & 1 \\
1 & 0 & 0 & 1
\end{pmatrix}
\end{align*}

\section*{Problem 2}
We can write the equations in matrix form as follows:
\begin{align*}
\begin{pmatrix}
2 & -3 & -1 & 1 \\
3 & 4 & -4 & -3 \\
0 & 17 & -5 & -9
\end{pmatrix}
\begin{pmatrix}
x_1 \\
x_2 \\
x_3 \\
x_4
\end{pmatrix}
=
\begin{pmatrix}
0 \\
0 \\
0
\end{pmatrix}
\end{align*}

To find the nontrivial solutions, we can row reduce the matrix to echelon form.
\begin{align*}
\begin{pmatrix}
2 & -3 & -1 & 1 \\
3 & 4 & -4 & -3 \\
0 & 17 & -5 & -9
\end{pmatrix} & r_2 = 2r_2 - 3r_1 \\
\begin{pmatrix}
2 & -3 & -1 & 1 \\
0 & 17 & -5 & -9 \\
0 & 17 & -5 & -9
\end{pmatrix} & r_3 = r_3 - r_2 \\
\begin{pmatrix}
2 & -3 & -1 & 1 \\
0 & 17 & -5 & -9 \\
0 & 0 & 0 & 0
\end{pmatrix}
\end{align*}

Which gives us the following system of equations:
\begin{align*}
2x_1 - 3x_2 - x_3 + x_4 &= 0 \\
17x_2 - 5x_3 - 9x_4 &= 0
\end{align*}

Let \(x_3 = \lambda\) and \(x_4 = \mu\) then we can express \(x_1\) and \(x_2\) in terms of \(\lambda\) and \(\mu\):
\begin{align*}
x_2 &= \frac{5\lambda + 9\mu}{17} \\
x_1 &= \frac{3x_2 + x_3 - x_4}{2} = \frac{3\left(\frac{5\lambda + 9\mu}{17}\right) + \lambda - \mu}{2}
\end{align*}
Thus, the general solution can be expressed as:
\begin{align*}
\begin{pmatrix}
\frac{3\left(\frac{5\lambda + 9\mu}{17}\right) + \lambda - \mu}{2} \\
\frac{5\lambda + 9\mu}{17} \\
\lambda \\
\mu
\end{pmatrix} & \lambda, \mu \in \mathbb{R}
\end{align*}

\section*{Problem 3}
\begin{align*}
    & \det\begin{pmatrix}
    a^2 + 1 & ab & ac \\
    ab & b^2 + 1 & bc \\
    ac & bc & c^2 + 1
    \end{pmatrix} \\
\end{align*}

Expand along the first row:
\begin{align*}
    & = (a^2 + 1) \det\begin{pmatrix}
    b^2 + 1 & bc \\
    bc & c^2 + 1
    \end{pmatrix} - ab \det\begin{pmatrix}
    ab & ac \\
    ac & c^2 + 1
    \end{pmatrix} + ac \det\begin{pmatrix}
    ab & b^2 + 1 \\
    ac & bc
    \end{pmatrix} \\
    &= (a^2 + 1)((b^2 + 1)(c^2 + 1) - b^2c^2) - ab(ab(c^2 + 1) - a^2c^2) + ac(ab^2c - ac(b^2 + 1)) \\
    &= (a^2 + 1)(b^2 + 1)(c^2 + 1) - (a^2 + 1)b^2c^2 - a^2b^2(c^2+1) + a^3bc^2 + a^2b^2c^2 - a^2c^2(b^2 + 1) \\
    &= (a^2b^2+a^2+b^2+1)(c^2 + 1) - (a^2 + 1)b^2c^2 - a^2b^2(c^2+1) + a^3bc^2 + a^2b^2c^2 - a^2c^2(b^2 + 1) \\
    &= a^2b^2c^2 +a^2b^2+a^2c^2+a^2+b^2c^2+b^2+c^2+1 - (a^2 + 1)b^2c^2 - a^2b^2(c^2+1) + a^3bc^2 + a^2b^2c^2 - a^2c^2(b^2 + 1) \\
    &= a^2 + b^2 + c^2 + 1
\end{align*}

\end{document}