\documentclass{article}
\usepackage{amsmath, amsthm, amssymb}
\usepackage{array}

\begin{document}
\section*{\huge Mathematics Homework Sheet 3}
\begin{flushright}
   \textbf{Author: Abdullah Oguz Topcuoglu \& Yousef Farag}
\end{flushright}

\begin{flushleft}
   \textbf{\Large Problem 1}
\end{flushleft}

\begin{flushleft}
   \textbf{\Large Problem 1 (a)}
\end{flushleft}

For i=0:
\begin{align*}
   f_1(-1) &= -1 \\
   f_1(0)  &= 0 \\
   f_1(1)  &= 0 \\
\end{align*}
Meaning that:
\[
   f_1(\{-1, 0, 1\}) = \{-1, 0, 0\} = \{-1, 0\}
\]
\\
Now lets take a look at the inverse:
\begin{align*}
   f_1(-1) &= -1 \\
   f_1(0)  &= 0 \\
   f_1(1)  &= 0 \\
   f_1(2)  &= 1 \\
\end{align*}
These are the only values we can get -1, 0, 1. Meaning that:
\[
   f_1^{-1}(\{-1, 0, 1\}) = \{-1, 0, 1, 2\}
\]
\\
Now, for i=2 (the second function):
\begin{align*}
   f_2(-1) &= -4 \\
   f_2(0)  &= -3 \\
   f_2(1)  &= -2 \\
\end{align*}
Meaning that:
\[
   f_2(\{-1, 0, 1\}) = \{-4, -3, -2\}
\]
\\
Now lets take a look at the inverse:
\begin{align*}
   f_2(2) &= -1 \\
   f_2(3) &= 0 \\
   f_2(4) &= 1 \\
\end{align*}
These are the only values we can get -1, 0, 1. Meaning that:
\[
   f_2^{-1}(\{-1, 0, 1\}) = \{2, 3, 4\}
\]
\\
Now, for i=3 (the third function):
\begin{align*}
   f_3(-1) &= -2 \\
   f_3(0)  &= 0 \\
   f_3(1)  &= 2 \\
\end{align*}
Meaning that:
\[
   f_3(\{-1, 0, 1\}) = \{-2, 0, 2\}
\]
\\
Now lets take a look at the inverse:
\begin{align*}
   f_3(x) & = -1 \text{, No such $x$ exists in the domain of $f_3$} \\
          & \text{In other words, } f_3^{-1}(\{-1\}) = \emptyset    \\
   f_3(0) & = 0                                                     \\
   f_3(x) & = 1 \text{, No such $x$ exists in the domain of $f_3$}  \\
          & \text{In other words, } f_3^{-1}(\{1\}) = \emptyset     \\
\end{align*}
These are the only values we can get -1, 0, 1. Meaning that:
\[
   f_3^{-1}(\{-1, 0, 1\}) = \{0\}
\]


\begin{flushleft}
   \textbf{\Large Problem 1 (b)}
\end{flushleft}

Lets start with \(f_1\): \\
\(f_1\) is not injective because it maps 0 and 1 to the same value, that is:
\[
   f_1(0) = f_1(1) = 0
\]
\\
\(f_1\) is surjective because it maps to all the values in the codomain. \\
Lets take an element from the codomain \(z \in Z\). \\
If \(z \leq 0\) then we can find an element in the domain of \(f_3\), \(x \in Z\) that maps to \(z\). Simply \(x = z\) works. \\
If \(z > 0\) then we can find an element in the domain of \(f_3\), \(x \in Z\) that maps to \(z\). Simply \(x = z + 1\) works. \\
\\
Now, lets take a look at \(f_2\): \\
\(f_2\) is injective because it maps each element in the domain to a unique element in the codomain, that is:
\begin{align*}
    & f_2(x) = f_2(y) \Rightarrow x = y \\
    & \\
    & f_2(x) = x - 3,\quad f_2(y) = y - 3    \\
    & x - 3 = y - 3 \Rightarrow x = y \\
\end{align*}
\\
\(f_2\) is surjective because it maps to all the values in the codomain. \\
Lets take an element from the codomain of \(f_2\), \(z \in Z\). \\
We cand find an element in the domain of \(f_2\), \(x \in Z\) that maps to \(z\). Simply \(x = z + 3\) works. \\
\\
Now, lets take a look at \(f_3\): \\
\(f_3\) is injective because it maps each element in the domain to a unique element in the codomain, that is:
\begin{align*}
    & f_3(x) = f_3(y) \Rightarrow x = y \\
    & \\
    & f_3(x) = 2x,\quad f_3(y) = 2y    \\
    & 2x = 2y \Rightarrow x = y \\
\end{align*}
\\
\(f_3\) is not surjective because it does not map to all the values in the codomain. \\
For example there is no element in the domain of \(f_3\) that maps to 1. Generally all the odd numbers are not in the range of \(f_3\). \\


\begin{flushleft}
   \textbf{\Large Problem 1 (c)}
\end{flushleft}

By looking at Problem 1 (b), \\
We see that \(f_1\) is not injective thus \(f_1\) is not bijective. \\
We see that \(f_2\) is injective and surjective thus \(f_2\) is bijective. \\
We see that \(f_3\) is not surjective thus \(f_3\) is not bijective. \\
\\
Inverse of \(f_2\):
\begin{align*}
   f_2: Z \rightarrow Z,& \quad x \rightsquigarrow x - 3 \\
   f_2^{-1}: Z \rightarrow Z,& \quad x \rightsquigarrow x + 3 \\
\end{align*}
\\


\end{document}