\documentclass{article}
\usepackage{amsmath, amsthm, amssymb}
\usepackage{array}

\begin{document}
\section*{\huge Mathematics Homework Sheet 6}
\begin{flushright}
   \textbf{Author: Abdullah Oguz Topcuoglu \& Yousef Farag}
\end{flushright}

\section*{Problem 1}
\section*{Problem 1 (a)}
We want to compute the following limit:
\[
   \lim_{n \rightarrow \infty} \frac{(n+1)^4(1 - 4n^3)^2}{(1+2n^2)^5}
\]
\\
The top part look somethin like this:
\[
   (n+1)^4(1 - 4n^3)^2 = 16n^{10} + \sum_{i = 0}^{i = 9} k_in^i
\]
And the bottom part look like this:
\[
   (1+2n^2)^5 = 32n^{10} + \sum_{i = 0}^{i = 9} k_in^i
\]
When we substitute these into the limit, we get:
\[
   \lim_{n \rightarrow \infty} \frac{16n^{10} + \sum_{i = 0}^{i = 9} k_in^i}{32n^{10} + \sum_{i = 0}^{i = 9} k_in^i}
\]
Divide the top and bottom by $n^{10}$:
\[
   \lim_{n \rightarrow \infty} \frac{16 + \sum_{i = 0}^{i = 9} k_in^{i-10}}{32 + \sum_{i = 0}^{i = 9} k_in^{i-10}}
\]
\[
   \frac{\lim_{n \rightarrow \infty}(16 + \sum_{i = 0}^{i = 9} k_in^{i-10})}{\lim_{n \rightarrow \infty}(32 + \sum_{i = 0}^{i = 9} k_in^{i-10})}
\]
\[
   \frac{16 + \sum_{i = 0}^{i = 9} k_i\lim_{n \rightarrow \infty}n^{i-10}}{32 + \sum_{i = 0}^{i = 9} k_i\lim_{n \rightarrow \infty}n^{i-10}}
\]
And we know that \(\lim_{n \rightarrow \infty} 1/n^i\) is zero for all \(i > 0\). Therefore, the limit is:
\[
   \frac{16}{32} = \frac{1}{2}
\]

\section*{Problem 1 (b)}
We want to compute the following limit:
\[
   \lim_{n \rightarrow \infty} \sqrt{n+1} - \sqrt{n}
\]
Multiply and divide by the conjugate:
\[
   \lim_{n \rightarrow \infty} \sqrt{n+1} - \sqrt{n} \cdot \frac{\sqrt{n+1} + \sqrt{n}}{\sqrt{n+1} + \sqrt{n}}
\]
\[
   \lim_{n \rightarrow \infty} \frac{n+1 - n}{\sqrt{n+1} + \sqrt{n}}
\]
\[
   \lim_{n \rightarrow \infty} \frac{1}{\sqrt{n+1} + \sqrt{n}}
\]
And observe that
\[
   \frac{1}{n^2} < \frac{1}{\sqrt{n+1} + \sqrt{n}} < \frac{1}{\sqrt{n}}
\]
when \(n > 10\) (10 is not a magic number, it is just a number that is big enough) 
and we only care about the tail of the sequences not the head.\\
And we know that:
\[
   \lim_{n \rightarrow \infty} \frac{1}{n^2} = 0
\]
\[
   \lim_{n \rightarrow \infty} \frac{1}{\sqrt{n}} = 0
\]
From the sandwich theorem, we can conclude that:
\[
   \lim_{n \rightarrow \infty} \frac{1}{\sqrt{n+1} + \sqrt{n}} = 0
\]

\section*{Problem 2}
\[
   a_n = (1 + \frac{1}{n})^n
\]
\[
   b_n = (1 + \frac{1}{n})^{n+1}
\]

\section*{Problem 2 (a)}
We want to prove that
\[
   \frac{a_{n + 1}}{a_n} = \left(1 - \frac{1}{(n+1)^2} \right)^{n+1} \frac{n+1}{n}
\]
Let's start
\begin{align*}
   \frac{a_{n+1}}{a_n} & = \frac{(1 + \frac{1}{n+1})^{n+1}}{(1 + \frac{1}{n})^n}                               \\
                        &= \frac{(n+2)^{n+1}n^n}{(n+1)^{2n+1}} \\
                        &= \frac{(n+2)^{n+1}n^{n+1}}{(n+1)^{2n+2}} \frac{n+1}{n} \\
                        &= \frac{(n+2)^{n+1}n^{n+1}}{((n+1)^2)^{n+1}} \frac{n+1}{n} \\
                        &= (\frac{(n+2)n}{(n+1)^2})^{n+1} \frac{n+1}{n} \\
                        &= (\frac{n^2+2n}{(n+1)^2})^{n+1} \frac{n+1}{n} \\
                        &= (\frac{n^2+2n+1 -1}{(n+1)^2})^{n+1} \frac{n+1}{n} \\
                        &= (\frac{n^2+2n+1}{(n+1)^2} - \frac{1}{((n+1)^2)})^{n+1} \frac{n+1}{n} \\
                        &= (1 - \frac{1}{(n+1)^2})^{n+1} \frac{n+1}{n} \\
\end{align*}
That's what we wanted to show. \\
\\
Now \(b_n\). We want to prove
\[
   \frac{b_n}{b_{n+1}} = \left(1 + \frac{1}{n(n+2)} \right)^{n+2} \frac{n}{n+1}
\]
Let's start
\begin{align*}
   \frac{b_n}{b_{n+1}} & = \frac{(1 + \frac{1}{n})^{n+1}}{(1 + \frac{1}{n+1})^{n+2}}                               \\
                        &= \frac{(n+1)^{2n+3}}{n^{n+1}(n+2)^{n+2}} \\
                        &= \frac{(n+1)^{2n+4}}{n^{n+2}(n+2)^{n+2}} \frac{n}{n+1} \\
                        &= \frac{((n+1)^2)^{n+2}}{n^{n+2}(n+2)^{n+2}} \frac{n}{n+1} \\
                        &= (\frac{(n+1)^2}{n(n+2)})^{n+2} \frac{n}{n+1} \\
                        &= (\frac{n^2 +2n + 1}{n(n+2)})^{n+2} \frac{n}{n+1} \\
                        &= (\frac{n(n+2) + 1}{n(n+2)})^{n+2} \frac{n}{n+1} \\
                        &= (1 + \frac{1}{n(n+2)})^{n+2} \frac{n}{n+1} \\
\end{align*}
That's what we wanted to show.


\end{document}