\documentclass{article}
\usepackage{amsmath, amsthm, amssymb}
\usepackage{array}

\begin{document}
\section*{\huge Mathematics Homework Sheet 10}
\begin{flushright}
   \textbf{Author: Abdullah Oguz Topcuoglu \& Yousef Farag}
\end{flushright}

\section*{Problem 1}

We want to compute the following using the power series of sin
\[
   \lim_{x \rightarrow 0} \frac{sin(x) - x}{x^3}
\]

Power series of sin is given as
\[
   sin(x) = \sum_{n=0}^{\infty} (-1)^n \frac{x^{2n+1}}{(2n+1)!}
\]

Let's insert this into the limit
\begin{align*}
   &\lim_{x \rightarrow 0} \frac{\sum_{n=0}^{\infty} (-1)^n \frac{x^{2n+1}}{(2n+1)!} - x}{x^3} \\
   &= \lim_{x \rightarrow 0} \frac{\sum_{n=1}^{\infty} (-1)^n \frac{x^{2n+1}}{(2n+1)!} - x + x}{x^3} \\
   &= \lim_{x \rightarrow 0} \frac{\sum_{n=1}^{\infty} (-1)^n \frac{x^{2n+1}}{(2n+1)!}}{x^3} \\
   &= \lim_{x \rightarrow 0} \sum_{n=1}^{\infty} (-1)^n \frac{x^{2n-2}}{(2n+1)!} \\
   &= \lim_{x \rightarrow 0} \sum_{n=2}^{\infty} (-1)^n \frac{x^{2n-2}}{(2n+1)!} - \frac{1}{3!} \\
   &= \sum_{n=2}^{\infty} (-1)^n \frac{\lim_{x \rightarrow 0} x^{2n-2}}{(2n+1)!} - \frac{1}{3!} \\
   &= 0 - \frac{1}{3!} \\
   &= - \frac{1}{6} \\
\end{align*}


\end{document}